theories/CompileCorrect.v
@@ -25,8 +25,99 @@ Fixpoint compile_value (Σ : EAst.global_declarations) (s : EWcbvEvalNamed.value
 
 Require Import FunctionalExtensionality.
 
+Lemma to_string_of_string s : 
+  String.to_string (String.of_string s) = s.
+Proof.
+  induction s; cbn.
+  - reflexivity.
+  - now rewrite Ascii.ascii_of_byte_of_ascii, IHs.
+Qed.
+
+Lemma of_string_to_string s : 
+  String.of_string (String.to_string s) = s.
+Proof.
+  induction s; cbn.
+  - reflexivity.
+  - now rewrite Ascii.byte_of_ascii_of_byte, IHs.
+Qed.
+
+Lemma lookup_map {A B} (f : A -> B) Γ x :
+  lookup (map (fun '(x0, v) => (x0, f v)) Γ) x = option_map f (lookup Γ x).
+Proof.
+  unfold lookup.
+  induction Γ as [ | []].
+  - reflexivity.
+  - cbn in *. change (String.eqb x i) with (eqb x i). destruct (eqb_spec x i).
+    + subst. reflexivity.
+    + eapply IHΓ.
+Qed.
+
+Lemma rev_spec {A} (l : list A) : MCList.rev l = rev l.
+Proof. 
+  unfold MCList.rev.
+  rewrite <- (app_nil_r (rev l)).
+  generalize (@nil A).
+  induction l; cbn; intros; try congruence.
+  rewrite IHl. now rewrite <- app_assoc.
+Qed.
+
+Lemma lookup_add a v Γ na :
+  lookup (add a v Γ) na = if na == a then Some v else lookup Γ na.
+Proof.
+  unfold add, lookup. cbn. change (String.eqb na a) with (na == a).
+  destruct (eqb_spec na a); congruence.
+Qed.
+
+Require Import Lia.
+
+Lemma lookup_multiple nms args Γ na :
+  List.length nms = List.length args ->
+  lookup (add_multiple nms args Γ) na = match find (fun x => na == fst x) (map2 pair nms args) with 
+                                        | Some (_, y) => Some y
+                                        | None => lookup Γ na
+                                        end.
+Proof.
+  intros Hlen. induction nms in args, Hlen |- *.
+  - destruct args; cbn in *; congruence.
+  - destruct args; cbn in *; try congruence.
+    rewrite lookup_add, IHnms. 2: cbn in *; lia.
+    destruct (eqb_spec na a).
+    + eauto.
+    + reflexivity.
+Qed.
+
+Lemma Mapply_eval globals locals (x : Malfunction.Ident.t)
+    (locals' : Malfunction.Ident.Map.t)
+    (e e2 : Malfunction.t) (v2 : SemanticsSpec.value)
+    (e1 : Malfunction.t) (v : SemanticsSpec.value) args :
+    SemanticsSpec.eval globals locals (Malfunction.Mapply (e1, args)) (Func (x, locals', e)) ->
+    SemanticsSpec.eval globals locals e2 v2 ->
+    SemanticsSpec.eval globals (Malfunction.Ident.Map.add x v2 locals') e v ->
+    SemanticsSpec.eval globals locals (Malfunction.Mapply (e1, args ++ [e2]))%list v.
+Proof.
+Admitted.  
+
+Lemma Mapply_u_spec f a :
+   (exists fn args, f = Malfunction.Mapply (fn, args) /\ Mapply_u f a = Malfunction.Mapply (fn, args ++ [a]))%list \/
+   (~ (exists fn args, f = Malfunction.Mapply (fn, args)) /\ Mapply_u f a = Malfunction.Mapply (f, [a])).
+Proof.
+  destruct f; cbn; firstorder try congruence.
+  left. destruct p. eauto.
+Qed.  
+
+Lemma lookup_env_In d Σ : 
+  EGlobalEnv.lookup_env Σ (fst d) = Some (snd d) -> In d Σ.
+Proof.
+  induction Σ; cbn in *.
+  - congruence.
+  - destruct (eqb_spec (fst d) (fst a)). intros [=]. destruct a, d; cbn in *; intuition auto.
+    left; subst; auto.
+    intros hl; specialize (IHΣ hl); intuition auto.
+Qed.
+
 Lemma compile_correct Σ s t Γ Γ' :
-  (forall na v, lookup Γ na = Some v -> Malfunction.Ident.Map.find (bytestring.String.to_string na) Γ' = compile_value Σ v) ->
+  (forall na, Malfunction.Ident.Map.find (bytestring.String.to_string na) Γ' =
+                match lookup Γ na with Some v => compile_value Σ v | _ => fail "notfound" end) ->
    EWcbvEvalNamed.eval Σ Γ s t ->
    SemanticsSpec.eval (compile_env Σ) Γ' (compile Σ s) (compile_value Σ t).
 Proof.
@@ -34,11 +125,60 @@ Proof.
   revert Γ' HΓ.
   induction Heval; intros Γ_ HΓ; simp compile; try rewrite <- !compile_equation_1.
   - (* variables *)
-    rewrite <- (HΓ _ _ e). econstructor.
+    specialize (HΓ na).
+    unfold EWcbvEvalNamed.lookup, lookup in *.
+    rewrite e in HΓ. rewrite <- HΓ.
+    econstructor. 
   - (* box app *)
     cbn. admit.
   - (* beta *)
-    admit.
+    destruct (Mapply_u_spec (compile Σ f) (compile Σ a)) as [(fn & arg & E & ->) | (E & ->) ].
+    + eapply Mapply_eval.
+      * rewrite <- E. cbn in IHHeval1. eauto.
+      * eauto.
+      * erewrite (functional_extensionality ((Malfunction.Ident.Map.add (String.to_string na) 
+             (compile_value Σ a')
+             (fun x : Malfunction.Ident.t =>
+              match
+                lookup (map (fun '(x0, v) => (x0, compile_value Σ v)) Γ')
+                  (String.of_string x)
+              with
+              | Some v => v
+              | None => fail "notfound"
+              end))) (fun na0 => match lookup (add na a' Γ') (String.of_string na0) with
+              | Some v => compile_value Σ v
+              | None => fail "notfound"
+              end)). eapply IHHeval3.
+        -- intros na0. unfold Malfunction.Ident.Map.find. now rewrite (of_string_to_string).
+        -- intros x.  unfold Malfunction.Ident.Map.find. rewrite lookup_add.
+           unfold Malfunction.Ident.Map.add. unfold Malfunction.Ident.eqb.
+           destruct (String.eqb_spec x (String.to_string na)).
+           ++ subst. rewrite of_string_to_string. now rewrite eqb_refl.
+           ++ destruct (eqb_spec (String.of_string x) na).
+              ** subst. rewrite to_string_of_string in n. congruence.
+              ** rewrite lookup_map. now destruct lookup.
+    + econstructor. cbn in *. eauto. eauto.
+      erewrite (functional_extensionality ((Malfunction.Ident.Map.add (String.to_string na) 
+             (compile_value Σ a')
+             (fun x : Malfunction.Ident.t =>
+              match
+                lookup (map (fun '(x0, v) => (x0, compile_value Σ v)) Γ')
+                  (String.of_string x)
+              with
+              | Some v => v
+              | None => fail "notfound"
+              end))) (fun na0 => match lookup (add na a' Γ') (String.of_string na0) with
+              | Some v => compile_value Σ v
+              | None => fail "notfound"
+              end)). eapply IHHeval3.
+        -- intros na0. unfold Malfunction.Ident.Map.find. now rewrite (of_string_to_string).
+        -- intros x.  unfold Malfunction.Ident.Map.find. rewrite lookup_add.
+           unfold Malfunction.Ident.Map.add. unfold Malfunction.Ident.eqb.
+           destruct (String.eqb_spec x (String.to_string na)).
+           ++ subst. rewrite of_string_to_string. now rewrite eqb_refl.
+           ++ destruct (eqb_spec (String.of_string x) na).
+              ** subst. rewrite to_string_of_string in n. congruence.
+              ** rewrite lookup_map. now destruct lookup.
   - (* lambda *)
     cbn.
     erewrite (functional_extensionality (fun x : Malfunction.Ident.t => match lookup (map (fun '(x0, v) => (x0, compile_value Σ v)) Γ) (String.of_string x) with
@@ -46,51 +186,109 @@ Proof.
                                        | None => fail "notfound"
                                        end)).
     econstructor.
-    intros x. unfold Malfunction.Ident.Map.find in *. 
-    admit.
-  - cbn. econstructor.
+    intros x. unfold Malfunction.Ident.Map.find in *.
+    specialize (HΓ (String.of_string x)).
+    rewrite to_string_of_string in HΓ.
+    rewrite HΓ, lookup_map.
+    destruct (lookup _ (String.of_string x)); eauto.
+  - (* let *) 
+    cbn. econstructor.
     + now eapply IHHeval1.
     + econstructor. eapply IHHeval2.
-      intros. unfold add, lookup in H. cbn in H.
+      intros. unfold add, lookup in *. cbn in *.
       change (String.eqb na0 na) with (na0 == na) in *.
       destruct (eqb_spec na0 na).
-      * inversion H; subst. unfold Malfunction.Ident.Map.add, Malfunction.Ident.Map.find, Malfunction.Ident.eqb.
+      * subst. unfold Malfunction.Ident.Map.add, Malfunction.Ident.Map.find, Malfunction.Ident.eqb.
         now rewrite String.eqb_refl.
       * unfold Malfunction.Ident.Map.add, Malfunction.Ident.Map.find, Malfunction.Ident.eqb.
         destruct (String.eqb_spec (String.to_string na0) (String.to_string na)).
-        -- admit.
-        -- eauto.
+        -- eapply (f_equal String.of_string) in e. rewrite !of_string_to_string in e.
+           congruence.
+        -- rewrite <- HΓ. reflexivity.
   - (* case *)
     replace ((Malfunction.Mswitch
-       (compile Σ discr,
-        mapi_InP brs 0
-          (fun (i : nat) (pat : list BasicAst.name * EAst.term) =>
-           let
-           '(nms0, b) as x := pat return (In x brs -> list Malfunction.case * Malfunction.t) in
-            fun _ : In (nms0, b) brs =>
-            ([Malfunction.Tag (Compile.int_of_nat i)],
-             Compile.Mapply_
-               (Compile.Mlambda_ (MCList.rev_map (fun nm : BasicAst.name => String.to_string (BasicAst.string_of_name nm)) nms0, compile Σ b),
-                MCList.mapi (fun (i0 : nat) (_ : BasicAst.name) => Malfunction.Mfield (Compile.int_of_nat i0, compile Σ discr)) (MCList.rev nms0)))))))
-              with (Mcase (compile Σ discr, map (fun '(brs, b) => (map (fun x => String.to_string (BasicAst.string_of_name x)) brs, compile Σ b)) brs)).
-    + eapply eval_case. all: admit.
+    (compile Σ discr,
+     mapi_InP brs 0
+       (fun (i : nat) (br0 : list BasicAst.name * EAst.term)
+          (_ : In br0 brs) =>
+        ([Malfunction.Tag (Compile.int_of_nat i)],
+         Compile.Mapply_
+           (Compile.Mlambda_
+              (MCList.rev_map
+                 (fun nm : BasicAst.name =>
+                  String.to_string (BasicAst.string_of_name nm)) 
+                 (fst br0), compile Σ (snd br0)),
+            MCList.mapi
+              (fun (i0 : nat) (_ : BasicAst.name) =>
+               Malfunction.Mfield (Compile.int_of_nat i0, compile Σ discr))
+              (MCList.rev (fst br0))))))))
+              with (Mcase (compile Σ discr, map (fun '(brs, b) => (MCList.rev_map (fun x => String.to_string (BasicAst.string_of_name x)) brs, compile Σ b)) brs)).
+    + destruct br as [br1 br2]. 
+      assert (pars = 0) as -> by todo "pars = 0".
+      rewrite skipn_O in *.
+      eapply eval_case. 
+      * cbn in *. eapply IHHeval1. eauto.
+      * rewrite nth_error_map, e0. cbn. reflexivity.
+      * todo "nodup".
+      * rewrite !map_length. cbn in *. rewrite MCList.rev_map_spec. rewrite rev_length, map_length. lia. 
+      * cbn in *. eapply IHHeval2. intros na.
+        rewrite lookup_multiple. 2: 
+        clear - HΓ f e2.        
+        induction br1 using rev_ind in nms, f, e2, br1, args |- *.
+        -- inversion f. subst. cbn. now eapply HΓ.
+        -- eapply Forall2_app_inv_l in f as (? & ? & ? & ? & ->). inversion H0. subst. inversion H5.
+           subst. rewrite rev_app_distr.
+           destruct args; rewrite app_length in e2; cbn in *; try lia.
+           rewrite MCList.rev_map_spec. rewrite map_app.
+           rewrite rev_app_distr. cbn.
+           unfold Malfunction.Ident.Map.add, Malfunction.Ident.eqb.
+           destruct (eqb_spec na y).
+           ++ subst. now rewrite String.eqb_refl.
+           ++ destruct (String.eqb_spec (String.to_string na) (String.to_string y)).
+              ** eapply (f_equal (String.of_string)) in e0. rewrite !of_string_to_string in e0. congruence.
+              ** rewrite <- IHbr1. 2: lia. 2: eauto.
+                 rewrite MCList.rev_map_spec. reflexivity.
+        -- eapply All_Forall.Forall2_length in f. rewrite rev_length. lia.
     + unfold Mcase. repeat f_equal.
       rewrite !MCList.mapi_map.
-      (* rewrite <- !mapi_InP_spec. *)
-      (* clear. generalize 0. induction brs; cbn; intros; simp mapi_InP. *)
-      (* * reflexivity. *)
-      (* * f_equal. destruct a. f_equal. *)
-      (*   rewrite !MCList.mapi_map. *)
-      (*   admit. *)
-      (*   eapply IHbrs. *)
-      (* *  *)
-      admit.
+      rewrite !mapi_InP_spec.
+      eapply MCList.mapi_ext. clear. intros n [nms br].
+      f_equal. change Mapply_ with Compile.Mapply_.
+      f_equal. change Mlambda_ with Compile.Mlambda_.
+      f_equal. cbn [fst snd].
+      rewrite MCList.rev_map_spec. cbn.
+      rewrite !MCList.mapi_rev. 
+      rewrite MCList.mapi_map.
+      rewrite rev_spec.
+      rewrite !MCList.mapi_rev. f_equal.
+      eapply MCList.mapi_ext. intros.
+      repeat f_equal. 
+      all: now rewrite map_length.
   - (* recursion *)
     admit.
   - (* fix *)
-    cbn. admit.
+    cbn.
+    destruct ((MCList.nth_error_Some' mfix (Datatypes.length mfix - idx - 1))) as [_ Hnth].
+    forward Hnth. todo "wf_fix".
+    econstructor.
+    + rewrite MCList.map_InP_spec. admit.
+    + econstructor. evar (v : SemanticsSpec.value).
+      replace (fail "ok") with v.
+      subst v. econstructor.
+      subst v. rewrite MCList.map_InP_spec.
+      erewrite nth_error_nth.
+      2: rewrite nth_error_map.
+      2: now rewrite (projT2 Hnth). cbn.
+      admit.
   - (* global *)
-    econstructor. 2: eauto. admit.
+    unshelve econstructor.
+    1: exact (compile Σ body).
+    2:{ eapply IHHeval. reflexivity. }
+    eapply in_flat_map.
+    unfold EGlobalEnv.declared_constant in *.    
+    eexists (_, _). split.
+    + eapply lookup_env_In. cbn. eauto.
+    + cbn. unfold compile_constant_decl. rewrite e. cbn. eauto.
   - (* constructor application *)
     cbn. econstructor.
     rewrite MCList.map_InP_spec, !map_app. cbn.
